charge and kripke

LTS.v
@@ -14,59 +14,79 @@ From ExtLib Require Import
      Structures.Maps
      Data.Map.FMapAList.
 
+From ChargeCore Require Import
+     Logics.ILogic
+     Logics.ILInsts.
+
 Section ETL.
 
   Variables (uid: Set) (atom: Set) (heap: Set).
 
+  (* Facts we learn and by whom  we learned them *)
   Inductive fact : Set :=
   | Ret: atom -> fact
-  | Knows: uid -> fact -> fact.
-  
-  (* Toy programming language executed by agents *)
+  | Says: uid -> fact -> fact.
+
+  Coercion Ret: atom >-> fact.
+
+  (* Toy programming language executed by each agent *)
   Inductive prog :=
   | Comp: prog
   | Send: uid -> fact -> prog
   | Recv: prog.
 
-  Definition db := list fact.
-  Definition trace := stream (uid * heap * prog * db)%type.
+  (* A single agent at one point in time *)
+  Record state := Agent {
+      user: uid;
+      mem: heap;
+      exe: prog;
+      db: list fact
+    }.
 
-  Variable init_trace: uid -> trace -> Prop.
+  (* A trace of an agent through time *)
+  Definition trace := stream state. 
 
+  (* Equality is decidable... *)
   Parameter eqdec_uid: RelDec (@eq uid).  
   Global Existing Instance eqdec_uid.
 
   Parameter eqdec_atom: RelDec (@eq atom).  
   Global Existing Instance eqdec_atom.
 
-  Global Instance eqdec_msg: RelDec (@eq fact) := {
+  Global Instance eqdec_fact: RelDec (@eq fact) := {
       rel_dec := fix rec(a b: fact) :=
         match a,b with
         | Ret a, Ret b => rel_dec a b
-        | Knows ua fa, Knows ub fb =>
+        | Says ua fa, Says ub fb =>
             andb (rel_dec ua ub) (rec fa fb)
         | _, _ => false
         end
     }.
 
-  Variable (transition: uid -> relation (heap*prog)).  
+  (* Each agent has a program -- a binary relation on (heap * prog) *)
+  Variable (transition: uid -> relation (heap*prog)).
+  
+  (* Transition function is functional & deterministic *)
   Variable (transition_determ: forall u s s' s'',
                transition u s s' ->
                transition u s s'' -> s' = s'').
 
-  (* Execute program Comp and produce new program p' and new heap st' *)
+  (* Toy Operational semantics of each agent *)
   Reserved Notation "a '-->' b" (at level 89).
-  Inductive cstep: uid * heap * prog * db -> uid * heap * prog * db -> Prop :=
-  | DoComp: forall st st' p' (d: db) (agent: uid),
-      transition agent (st, Comp) (st', p') ->
-      cstep (agent, st, Comp, d) (agent, st', p', d)
+  Inductive cstep: state -> state -> Prop :=
+  | DoComp: forall st st' p' d (a: uid),
+      transition a (st, Comp) (st', p') ->
+      cstep (Agent a st Comp d) (Agent a st' p' d)
   where "a '-->' b" := (cstep a b).
 
-  (** A distributed system is a list of traces *)
+  (* A distributed system is a list of traces *)
   Definition system := list trace.
-  
+
+  (* With an initial state *)
+  Variable init_system: system -> Prop.
+
+  (* Network (system) semantics *)
   Reserved Notation "a '==>' b" (at level 90).
-  
   Inductive step: system -> system  -> Prop :=
   | LocalStep: forall a a' past hds tls,
     a --> a' ->
@@ -76,41 +96,92 @@ Section ETL.
       transition ua (ha, Send ub m) (ha', pa) ->
       transition ub (hb, Recv) (hb', pb) ->
       hds
-      ++ [ Continue  (ua, ha, Send ub m, dba) past ]
+      ++ [ Continue  (Agent ua ha (Send ub m) dba) past ]
       ++ mid
-      ++ [ Continue (ub, hb, Recv, dbb) past' ]
+      ++ [ Continue (Agent ub hb Recv dbb) past' ]
       ++ tls ==>
       hds
-      ++ [ Continue (ua, ha, pa, dba)
-             (Continue (ua, ha', Send ub m, dba) past) ]
+      ++ [ Continue (Agent ua ha pa dba)
+             (Continue (Agent ua ha' (Send ub m) dba) past) ]
       ++ mid
-      ++ [ Continue (ub, hb', pb, (Knows ua m) :: dbb)
-             (Continue (ub, hb, Recv, dbb) past') ]
+      ++ [ Continue (Agent ub hb' pb (Says ua m :: dbb))
+             (Continue (Agent ub hb Recv dbb) past') ]
       ++ tls
   where "a '==>' b" := (step a b).
 
+  (* Transitive-reflexive closure of step *)
   Notation "a '==>*' b" := (step ^* a b) (at level 40).
 
-  Notation traceProp := (trace -> Prop).
-  Notation stateProp := (uid * heap * prog * db -> Prop).
+  (***************** Logic ********************)
+  Definition systemProp := (system -> Prop).
+  Definition traceProp := (trace -> Prop).
+  Definition stateProp := (state -> Prop).
+  Definition atomProp := (atom -> Prop).
+  Definition factProp := (fact -> Prop).
 
-  Definition and (P Q : traceProp) : traceProp :=
-    fun str => P str /\ Q str.
+  (***************** Focusing different parts of the logic ******************)
+  Definition system2trace(P: systemProp): traceProp :=
+    fun str => P ([str]).
 
-  Definition and_state (P Q : stateProp) : stateProp :=
-    fun s => P s /\ Q s.
+  Definition state2trace(P: stateProp): traceProp :=
+    fun str => P (hd str).
 
-  Definition or (P Q : traceProp) : traceProp :=
-    fun str => P str \/ Q str.
+  Definition fact2state(P: factProp): stateProp :=
+    fun st => List.Exists P (db st).
 
-  Definition or_state (P Q : stateProp) : stateProp :=
-    fun s => P s \/ Q s.
+  Inductive atom2fact(P: atomProp): factProp :=
+    RetValid: forall a, P a -> atom2fact P (Ret a).
+  
+  (********************** Path restriction *******************)
+  Definition restrict(users: list uid)(P: systemProp): systemProp :=
+    fun s =>
+      P (List.filter (fun str => List.existsb (fun a => rel_dec (user (hd str)) a) users) s).
+  
+  Declare Custom Entry etl.
+  Declare Scope etl_scope.
 
-  (** How to compose 'implies' and '==>*' *)
-  Definition leads_to_state (P Q : stateProp) : Prop :=
-    forall s t , P s -> s --> t -> Q t.
+  Notation "<{ a '|-' e }>" :=
+    (restrict a e)
+      (at level 0, a constr, e custom etl at level 99) : etl_scope.
 
-  (****************************** Temporal basic operators *************************)
+  Notation "( x )" := x (in custom etl, x at level 99) : etl_scope.
+  Notation "x" := x (in custom etl at level 0, x constr at level 0) : etl_scope.
+
+  (********************** Path quantification now *************************)
+  Definition forall_agents(P: traceProp): systemProp :=
+    fun s => List.Forall (fun str => P str) s.
+  
+  Definition exists_agent(P: traceProp): systemProp :=
+    fun s => List.Exists (fun str => P str) s.
+
+  Definition forall_now(P: stateProp): systemProp :=
+    fun s => List.Forall (fun str => P (hd str)) s.
+  
+  Definition exist_now(P: stateProp): systemProp :=
+    fun s => List.Exists (fun str => P (hd str)) s.
+
+  Coercion forall_agents: traceProp >-> systemProp.
+  Coercion system2trace: systemProp >-> traceProp.
+  
+  (***************** Property impled by big-step *********************)
+  Definition leads_to (P Q : systemProp) : Prop :=
+    forall s t , P s -> s ==>* t -> Q t.
+
+  (***************** All the intuitionistic logics! *****************)
+  Global Instance ILogicOps_systemProp : ILogicOps systemProp := _.
+
+  Notation "x /\ y"   := (land x y) (in custom etl at level 50, left associativity).
+  Notation "x \/ y"   := (lor x y) (in custom etl at level 50, left associativity).
+  Notation "'True'"   := (ltrue: systemProp) (in custom etl at level 0).
+  Notation "'False'"  := (lfalse: systemProp) (in custom etl at level 0).
+  Notation "x -> y"   := (limpl x y) (in custom etl at level 50, left associativity).
+  Notation "x <-> y"   :=
+    (land (limpl x y) (limpl y x)) (in custom etl at level 50, left associativity).
+  Notation "~ a"      := (limpl a lfalse) (in custom etl at level 40).
+  Notation "'forall' a ',' b" := (lforall a b) (in custom etl at level 80).
+  Notation "'exists' a ',' b" := (lexists a b) (in custom etl at level 80).
+    
+  (************** Temporal basic operators (stream) ********************)
   Definition next (P : traceProp) : traceProp :=
     fun str => P (tl str).
 
@@ -137,31 +208,71 @@ Section ETL.
     forall s (str : trace),
       P (Continue s str) -> unless P Q str -> unless P Q (Continue s str).
 
+  Notation "[] a"  := (always a)  (in custom etl at level 90).
+  Notation "<> a" := (eventually a) (in custom etl at level 90).
 
-(****************************** Temporal derived operators ***********************)
+  (****************************** Temporal derived operators ***********************)
+  Definition infinitely_often (P : traceProp) : 
+    traceProp := always (eventually P).
 
-Definition infinitely_often (P : traceProp) : 
-  traceProp := always (eventually P).
+  Definition implies (P Q : traceProp) : traceProp :=
+    always (fun str : trace => P str -> Q str).
 
-Definition implies (P Q : traceProp) : traceProp :=
-  always (fun str : trace => P str -> Q str).
+  Definition is_followed (P Q : traceProp) (str : trace) : Prop :=
+    P str -> eventually Q str.
+  
+  Definition is_always_followed (P Q : traceProp) : 
+    traceProp := always (is_followed P Q).
 
-Definition is_followed (P Q : traceProp) (str : trace) : Prop :=
-  P str -> eventually Q str.
+  Definition eventually_permanently (P : traceProp) : 
+    traceProp := eventually (always P).
 
-Definition is_always_followed (P Q : traceProp) : 
-  traceProp := always (is_followed P Q).
+  Definition once_always (P Q : traceProp) : traceProp :=
+    implies P (always Q).
 
-Definition eventually_permanently (P : traceProp) : 
-  traceProp := eventually (always P).
+  Definition leads_to_via (P Q R : traceProp) : 
+    traceProp := implies P (until Q R).
 
-Definition once_always (P Q : traceProp) : traceProp :=
-  implies P (always Q).
+  Definition once_until (P Q : traceProp) : traceProp :=
+    leads_to_via P P Q.
 
-Definition leads_to_via (P Q R : traceProp) : 
-  traceProp := implies P (until Q R).
+  (****************************** Epistemic Knowledge operators ***********************)
+  Fixpoint powerset{T}(l: list T): list (list T) :=
+    match l with
+    | nil => [nil]
+    | x :: xs =>
+      let ps := powerset xs in
+      ps ++ List.map (fun ss => x :: ss) ps
+    end.
 
-Definition once_until (P Q : traceProp) : traceProp :=
-  leads_to_via P P Q.
+  Definition is_rumor(f: fact): bool :=
+     match f with
+     | Says _  _ => true
+     | Ret _ => false
+     end.
+
+  Fixpoint trust(f: fact): atom :=
+     match f with
+     | Says _ f => trust f
+     | Ret a => a
+     end.
+  
+  Definition rumors(l: list fact): list fact :=    
+    List.filter is_rumor l.
+
+  Fixpoint possible_worlds(db: list fact): list (list atom) :=
+    List.map (fun l => List.map trust l) (powerset db).
+
+  Definition over_db(st: state)(d: list atom): state :=
+    match st with
+    | Agent u h p l => Agent u h p (List.map Ret d)
+    end.
+
+  (* For this point in time, knowledge means to consider
+     something valid in all possible worlds (Kripke) *)
+  Definition knowledge(P: stateProp): stateProp :=
+    fun st => forall w, In w (possible_worlds (db st)) ->
+                P st <-> P (over_db st w).
+
 
 End ETL.
